 **Question 1(a)**:


### **Given Identities to Prove:**

1. $e^{i\theta} + e^{-i\theta} = 2\cos\theta$
2. $e^{i\theta} - e^{-i\theta} = 2i\sin\theta$

 

### **Using Euler’s Formula:**

Euler's formulas are:

$$
e^{i\theta} = \cos\theta + i\sin\theta \quad \text{and} \quad e^{-i\theta} = \cos\theta - i\sin\theta
$$

 

### **1. Proving $e^{i\theta} + e^{-i\theta} = 2\cos\theta$:**

Add the two expressions:

$$
e^{i\theta} + e^{-i\theta} = (\cos\theta + i\sin\theta) + (\cos\theta - i\sin\theta)
$$

$$
= 2\cos\theta
$$

✅ **Hence proved.**

 

### **2. Proving $e^{i\theta} - e^{-i\theta} = 2i\sin\theta$:**

Subtract the two expressions:

$$
e^{i\theta} - e^{-i\theta} = (\cos\theta + i\sin\theta) - (\cos\theta - i\sin\theta)
$$

$$
= 2i\sin\theta
$$

✅ **Hence proved.**

 

### **Graphical Interpretation (Brief)**:

* The function $e^{i\theta}$ traces a point on the **unit circle** in the complex plane.
* $e^{i\theta} + e^{-i\theta}$ gives a real number, aligning with the **x-axis**: it's twice the projection (cosine) on the real axis.
* $e^{i\theta} - e^{-i\theta}$ gives a purely imaginary number, aligning with the **y-axis**: it's twice the sine value scaled by $i$, i.e., projection on the imaginary axis.

![image](https://github.com/user-attachments/assets/9217eb83-4c85-4deb-9a05-1f7b08ba5fa0)


## **1(b) Show that if $z(t) = e^{it}$ represents the position vector, then $iz(t)$ is the perpendicular velocity vector.**

### **Step 1: Position Vector**

$$
z(t) = e^{it} = \cos t + i\sin t
$$

This represents a point moving along the **unit circle** (since $|z| = 1$) in the complex plane.

### **Step 2: Differentiate to find velocity**

$$
\frac{dz}{dt} = \frac{d}{dt} (\cos t + i\sin t) = -\sin t + i\cos t
$$

Now multiply $z(t)$ by $i$:

$$
i z(t) = i(\cos t + i\sin t) = i\cos t - \sin t = -\sin t + i\cos t
$$

➡️ **So $iz(t) = \frac{dz}{dt}$**.

This shows:

* $iz(t)$ is tangent (i.e., the velocity vector).
* It is **perpendicular** to $z(t)$, because multiplying by $i$ in the complex plane rotates any vector by $90^\circ$ counterclockwise.

✅ **Hence proved.**

![image](https://github.com/user-attachments/assets/4156df04-a693-4eef-b4a1-ebc319f05816)


## **1(c) If $z = (-5 - 5i)^{1/3}$, express in polar form and find all values.**

### **Step 1: Convert to polar form**

Given:

$$
z_0 = -5 - 5i
$$

* **Modulus**:

$$
r = |z_0| = \sqrt{(-5)^2 + (-5)^2} = \sqrt{50} = 5\sqrt{2}
$$

* **Argument**:

$$
\theta = \arg(z_0) = \tan^{-1}\left(\frac{-5}{-5}\right) = \tan^{-1}(1) = \frac{\pi}{4}
$$

But since $z_0$ lies in **3rd quadrant**, add $\pi$:

$$
\theta = \pi + \frac{\pi}{4} = \frac{5\pi}{4}
$$

So,

$$
z_0 = 5\sqrt{2} \text{cis} \left( \frac{5\pi}{4} \right)
$$

 

### **Step 2: Cube roots**

General formula:

$$
z_k = r^{1/3} \text{cis} \left( \frac{\theta + 2k\pi}{3} \right), \quad k = 0, 1, 2
$$

Here,

* $r^{1/3} = (5\sqrt{2})^{1/3}$
* $\theta = \frac{5\pi}{4}$

Now compute:

$$
z_0 = (5\sqrt{2})^{1/3} \text{cis} \left( \frac{5\pi}{12} \right)
$$

$$
z_1 = (5\sqrt{2})^{1/3} \text{cis} \left( \frac{5\pi}{12} + \frac{2\pi}{3} \right) = \text{cis} \left( \frac{13\pi}{12} \right)
$$

$$
z_2 = (5\sqrt{2})^{1/3} \text{cis} \left( \frac{5\pi}{12} + \frac{4\pi}{3} \right) = \text{cis} \left( \frac{21\pi}{12} \right) = \text{cis} \left( \frac{7\pi}{4} \right)
$$

✅ So the **three cube roots** are:

$$
(5\sqrt{2})^{1/3} \text{cis} \left( \frac{5\pi}{12} \right),\quad (5\sqrt{2})^{1/3} \text{cis} \left( \frac{13\pi}{12} \right),\quad (5\sqrt{2})^{1/3} \text{cis} \left( \frac{7\pi}{4} \right)
$$

 

## **1(d) Given $v(x, y) = \cos x \sinh y$, prove it satisfies Laplace’s Equation and find $u(x, y)$ such that $f = u + iv$ is analytic.**

 

### **Step 1: Laplace’s Equation**

Laplace’s equation:

$$
\frac{\partial^2 v}{\partial x^2} + \frac{\partial^2 v}{\partial y^2} = 0
$$

Compute derivatives:

* $\frac{\partial v}{\partial x} = -\sin x \sinh y$

* $\frac{\partial^2 v}{\partial x^2} = -\cos x \sinh y$

* $\frac{\partial v}{\partial y} = \cos x \cosh y$

* $\frac{\partial^2 v}{\partial y^2} = \cos x \sinh y$

So:

$$
\frac{\partial^2 v}{\partial x^2} + \frac{\partial^2 v}{\partial y^2} = -\cos x \sinh y + \cos x \sinh y = 0
$$

✅ Hence, **$v(x, y)$ satisfies Laplace’s Equation.**

 

### **Step 2: Use Cauchy-Riemann to find $u(x, y)$**

Cauchy-Riemann Equations:

$$
\frac{\partial u}{\partial x} = \frac{\partial v}{\partial y} = \cos x \cosh y \\
\frac{\partial u}{\partial y} = -\frac{\partial v}{\partial x} = \sin x \sinh y
$$

Integrate $\frac{\partial u}{\partial x}$ w\.r.t. $x$:

$$
u(x, y) = \int \cos x \cosh y \, dx = \sin x \cosh y + h(y)
$$

Differentiate this w\.r.t. $y$:

$$
\frac{\partial u}{\partial y} = \sin x \sinh y + h'(y)
$$

Set equal to second C-R result:

$$
\sin x \sinh y + h'(y) = \sin x \sinh y \Rightarrow h'(y) = 0 \Rightarrow h(y) = C
$$

So,

$$
u(x, y) = \sin x \cosh y + C
$$

✅ Therefore, the **analytic function** is:

$$
f(x + iy) = u(x, y) + iv(x, y) = \sin x \cosh y + i \cos x \sinh y
$$


## **2(a) Expand**

$$
f(z) = \frac{z}{(z+1)(z+2)}
$$

### into Laurent series valid for:

 

### **(i) $|z| < 2$**

We express $f(z)$ in partial fractions:

$$
\frac{z}{(z+1)(z+2)} = \frac{A}{z+1} + \frac{B}{z+2}
$$

Multiply both sides by $(z+1)(z+2)$:

$$
z = A(z+2) + B(z+1)
$$

Substitute:

* $z = -2$: $-2 = A(0) + B(-1) \Rightarrow B = 2$
* $z = -1$: $-1 = A(1) + B(0) \Rightarrow A = -1$

So:

$$
f(z) = \frac{-1}{z+1} + \frac{2}{z+2}
$$

Now, expand each term as a power series centered at 0.

 

**For $\frac{1}{z+1}$:**

$$
\frac{1}{z+1} = \frac{1}{1 + z} = \sum_{n=0}^{\infty} (-1)^n z^n \quad \text{for } |z| < 1
$$

But we need $|z| < 2$, so this is valid and converges for $|z| < 1$, **but not up to 2**.

So instead, write using geometric series for a wider range.

Let’s express:

$$
\frac{1}{z+1} = \frac{1}{1 + z} = \sum_{n=0}^{\infty} (-z)^n, \quad |z| < 1
$$

$$
\frac{1}{z+2} = \frac{1}{2(1 + \frac{z}{2})} = \frac{1}{2} \sum_{n=0}^{\infty} (-1)^n \left(\frac{z}{2}\right)^n = \sum_{n=0}^{\infty} \frac{(-1)^n z^n}{2^{n+1}}, \quad |z| < 2
$$

Then:

$$
f(z) = -\sum_{n=0}^{\infty} (-z)^n + 2\sum_{n=0}^{\infty} \frac{(-1)^n z^n}{2^{n+1}}
$$

 

### **(ii) $1 < |z| < 2$**

Here we must write one term as a Laurent series with negative powers.

Use:

$$
\frac{1}{z+1} = \frac{1}{z(1 + \frac{1}{z})} = \frac{1}{z} \cdot \sum_{n=0}^\infty (-1)^n z^{-n} = \sum_{n=1}^\infty (-1)^{n-1} z^{-n}
$$

$$
\frac{1}{z+2} = \frac{1}{2(1 + \frac{z}{2})} = \sum_{n=0}^{\infty} \frac{(-1)^n z^n}{2^{n+1}}, \quad |z| < 2
$$

Hence:

$$
f(z) = -\sum_{n=1}^\infty (-1)^{n-1} z^{-n} + 2\sum_{n=0}^{\infty} \frac{(-1)^n z^n}{2^{n+1}}
$$

✅ **Done for both regions.**

 

## **2(b) Find Laurent Series and Residue**

Given:

$$
f(z) = \frac{e^z - 1 - z}{z^3}, \quad z = 0
$$

### Step 1: Taylor expansion of $e^z$:

$$
e^z = 1 + z + \frac{z^2}{2!} + \frac{z^3}{3!} + \cdots
$$

Then:

$$
e^z - 1 - z = \frac{z^2}{2} + \frac{z^3}{6} + \frac{z^4}{24} + \cdots
$$

So:

$$
f(z) = \frac{e^z - 1 - z}{z^3} = \frac{z^2}{2z^3} + \frac{z^3}{6z^3} + \frac{z^4}{24z^3} + \cdots
= \frac{1}{2z} + \frac{1}{6} + \frac{z}{24} + \cdots
$$

### Type of Singularity:

* Since there's a term $\frac{1}{z}$, this is a **simple pole** at $z = 0$.

### Residue:

* The coefficient of $\frac{1}{z}$ is the **residue**.
* ✅ Residue = $\frac{1}{2}$

 

## **2(c) Evaluate**

$$
\oint_C \frac{e^{zt}}{z^2 + 1} \, dz, \quad t > 0, \quad C: |z| = 3
$$

### Step 1: Poles of integrand

$$
z^2 + 1 = 0 \Rightarrow z = \pm i
$$

These are **simple poles** inside $|z| = 3$.

 

### Step 2: Residues at poles

Let’s find residue at $z = i$:

$$
\text{Res}_{z=i} = \lim_{z \to i} (z - i) \frac{e^{zt}}{(z + i)(z - i)} = \frac{e^{it}}{2i}
$$

At $z = -i$:

$$
\text{Res}_{z=-i} = \frac{e^{-it}}{-2i}
$$

 

### Step 3: Use Residue Theorem

$$
\oint_C \frac{e^{zt}}{z^2 + 1} dz = 2\pi i \left( \frac{e^{it}}{2i} + \frac{e^{-it}}{-2i} \right)
= 2\pi i \left( \frac{e^{it} - e^{-it}}{2i} \right)
= 2\pi i \cdot \sin t
$$

✅ Final answer:

$$
\oint_C \frac{e^{zt}}{z^2 + 1} dz = 2\pi \sin t
$$

 

## **2(d) Show that**

$$
\int_0^{\infty} \frac{\cos(mx)}{x^2 + a^2} dx = \frac{\pi e^{-ma}}{2a}
$$

Use the complex integral trick:

$$
\int_{-\infty}^\infty \frac{e^{imx}}{x^2 + a^2} dx
$$

This evaluates to:

$$
\frac{\pi}{a} e^{-ma} \quad \text{(standard result using contour integration)}
$$

Now take **real part**:

$$
\int_{-\infty}^\infty \frac{\cos(mx)}{x^2 + a^2} dx = \frac{\pi}{a} e^{-ma}
$$

Now restrict to $[0, \infty)$:

$$
\int_0^{\infty} \frac{\cos(mx)}{x^2 + a^2} dx = \frac{1}{2} \cdot \frac{\pi}{a} e^{-ma}
= \frac{\pi e^{-ma}}{2a}
$$

✅ Hence proved.


## **3(a) Find all values of $z$ such that $z^5 = -32$, and locate them on the complex plane.**

### Step 1: Express RHS in polar form

$$
-32 = 32 \cdot \text{cis}(\pi)
$$

Where $\text{cis}(\theta) = \cos \theta + i \sin \theta$

So,

$$
z^5 = 32 \text{cis}(\pi)
$$

Take fifth roots:

$$
z = 32^{1/5} \cdot \text{cis} \left( \frac{\pi + 2k\pi}{5} \right), \quad k = 0, 1, 2, 3, 4
$$

$$
32^{1/5} = 2
$$

Thus, the five roots are:

$$
z_k = 2 \cdot \text{cis} \left( \frac{\pi + 2k\pi}{5} \right), \quad k = 0, 1, 2, 3, 4
$$

These are:

* $z_0 = 2 \cdot \text{cis} \left( \frac{\pi}{5} \right)$
* $z_1 = 2 \cdot \text{cis} \left( \frac{3\pi}{5} \right)$
* $z_2 = 2 \cdot \text{cis} \left( \pi \right) = -2$
* $z_3 = 2 \cdot \text{cis} \left( \frac{7\pi}{5} \right)$
* $z_4 = 2 \cdot \text{cis} \left( \frac{9\pi}{5} \right)$

 

### Step 2: Plot on complex plane

These 5 roots lie on a **circle of radius 2** centered at the origin, spaced **72° apart** (since $\frac{2\pi}{5} = 72^\circ$).

They form a regular **pentagon** inscribed in the circle, one vertex on the negative real axis.

✅ **Done.**

 

## **3(b) Represent graphically the set of values of $z$ for which:**

$$
\left| \frac{z - 3}{z + 3} \right| = 2
$$

 

### Step 1: Geometric Interpretation

This is of the form:

$$
\left| \frac{z - z_1}{z - z_2} \right| = k
$$

It represents an **Apollonius circle** – the set of all points $z$ for which the ratio of distances to two fixed points is constant.

Here:

* $z_1 = 3$
* $z_2 = -3$
* $k = 2$

So, the locus is:

$$
\frac{|z - 3|}{|z + 3|} = 2
$$

This is the set of points in the complex plane for which the distance to $z = 3$ is **twice** the distance to $z = -3$.

 

### Step 2: Equation of Apollonius Circle

Let $z = x + iy$. Then:

$$
\frac{\sqrt{(x - 3)^2 + y^2}}{\sqrt{(x + 3)^2 + y^2}} = 2
$$

Square both sides:

$$
\frac{(x - 3)^2 + y^2}{(x + 3)^2 + y^2} = 4
$$

Cross-multiply:

$$
(x - 3)^2 + y^2 = 4[(x + 3)^2 + y^2]
$$

Expand both sides:

LHS:

$$
x^2 - 6x + 9 + y^2
$$

RHS:

$$
4(x^2 + 6x + 9 + y^2) = 4x^2 + 24x + 36 + 4y^2
$$

Now subtract both sides:

$$
x^2 - 6x + 9 + y^2 = 4x^2 + 24x + 36 + 4y^2
$$

Bring all terms to one side:

$$
x^2 - 6x + 9 + y^2 - 4x^2 - 24x - 36 - 4y^2 = 0
$$

$$
-3x^2 -30x -3y^2 -27 = 0
$$

Divide through by -3:

$$
x^2 + 10x + y^2 + 9 = 0
$$

Complete the square:

$$
(x + 5)^2 - 25 + y^2 + 9 = 0
\Rightarrow (x + 5)^2 + y^2 = 16
$$

 

### Final Answer:

✅ The locus is a **circle** with:

* **Center**: $(-5, 0)$
* **Radius**: $4$

![image](https://github.com/user-attachments/assets/ed3a607f-19d2-4ec3-b852-ce5daff3741d)

