
## ✅ **Question 1(a): Define Laplace Transform with Applications**

### **Definition**:

The **Laplace Transform** of a function $f(t)$, defined for all $t \geq 0$, is given by:

$$
\mathcal{L}\{f(t)\} = F(s) = \int_0^\infty e^{-st}f(t)\,dt
$$

Where:

* $f(t)$ is a time-domain function.
* $F(s)$ is the Laplace-transformed function in the **frequency domain**.
* $s$ is a complex number.

---

### **Real-life Applications**:

1. **Electrical Engineering**: Analysis of RLC circuits using transfer functions.
2. **Control Systems**: To model dynamic systems and design controllers.
3. **Mechanical Engineering**: For vibration analysis and system modeling.
4. **Differential Equations**: Solves linear ODEs with initial conditions.
5. **Signal Processing**: Used for system response and filtering in time domain.

---

## ✅ **Question 1(b): Laplace Transforms**

---

### **(i)** $F(t) = e^{3t}(2\cos 5t - 3\sin 5t)$

**Use**:

$$
\mathcal{L}\{e^{at}\cos(bt)\} = \frac{s - a}{(s - a)^2 + b^2},\quad \mathcal{L}\{e^{at}\sin(bt)\} = \frac{b}{(s - a)^2 + b^2}
$$

Break it:

* $\mathcal{L}\{e^{3t}\cos(5t)\} = \frac{s - 3}{(s - 3)^2 + 25}$
* $\mathcal{L}\{e^{3t}\sin(5t)\} = \frac{5}{(s - 3)^2 + 25}$

Final result:

$$
\mathcal{L}\{F(t)\} = 2 \cdot \frac{s - 3}{(s - 3)^2 + 25} - 3 \cdot \frac{5}{(s - 3)^2 + 25}
= \frac{2(s - 3) - 15}{(s - 3)^2 + 25}
$$

---

### **(ii)** $F(t) = t^2 \sin(at)$

**Use**:

$$
\mathcal{L}\{t^n \sin(at)\} = \frac{n! \cdot a}{(s^2 + a^2)^{n + 1}}
$$

For $n = 2$:

$$
\mathcal{L}\{t^2 \sin(at)\} = \frac{2! \cdot a}{(s^2 + a^2)^3} = \frac{2a}{(s^2 + a^2)^3}
$$

---

### **(iii)**

$$
F(t) =
\begin{cases}
\sin t, & 0 < t < \pi \\
0, & \pi < t < 2\pi
\end{cases}
$$

This is a piecewise function. Use the **unit step function**:

$$
F(t) = \sin t \cdot [u(t) - u(t - \pi)]
$$

Now apply Laplace transform:

$$
\mathcal{L}\{f(t)[u(t) - u(t - \pi)]\} = \mathcal{L}\{\sin t\} - e^{-\pi s} \mathcal{L}\{\sin(t + \pi)\}
$$

$$
= \frac{1}{s^2 + 1} - e^{-\pi s} \cdot \frac{\sin(t + \pi)} \Rightarrow \sin(t + \pi) = -\sin t
$$

So:

$$
\mathcal{L}\{F(t)\} = \frac{1}{s^2 + 1} + \frac{e^{-\pi s}}{s^2 + 1}
= \frac{1 + e^{-\pi s}}{s^2 + 1}
$$

---

## ✅ **Question 1(c): Solve System Using Laplace Transform**

Given:

$$
\frac{dx}{dt} = 2x - 3y,\quad \frac{dy}{dt} = y - 2x,\quad x(0)=8,\ y(0)=3
$$

Take Laplace transforms:
Let $X(s) = \mathcal{L}\{x(t)\},\ Y(s) = \mathcal{L}\{y(t)\}$

Then:

$$
sX(s) - x(0) = 2X(s) - 3Y(s) \Rightarrow sX(s) - 8 = 2X(s) - 3Y(s) \quad \text{(1)}
$$

$$
sY(s) - y(0) = Y(s) - 2X(s) \Rightarrow sY(s) - 3 = Y(s) - 2X(s) \quad \text{(2)}
$$

Rewriting:

* Eq (1): $(s - 2)X(s) + 3Y(s) = 8$
* Eq (2): $2X(s) + (1 - s)Y(s) = -3$

---

### Solve the linear system:

Multiply (1) by $1 - s$, (2) by 3, then eliminate.

You get:

$$
X(s) = \frac{8(s - 1) - 9}{(s - 2)(s - 1) + 6}
= \frac{8s - 17}{s^2 - 3s + 8}
$$

Now:

$$
x(t) = \mathcal{L}^{-1}\left\( \frac{8s - 17}{s^2 - 3s + 8} \right\)
$$

Complete the square:

$$
s^2 - 3s + 8 = (s - \frac{3}{2})^2 + \frac{23}{4}
$$

Use inverse Laplace formulas to express the result as:

$$
x(t) = Ae^{\frac{3}{2}t} \cos\left(\sqrt{\frac{23}{4}}t\right) + Be^{\frac{3}{2}t} \sin\left(\sqrt{\frac{23}{4}}t\right)
$$

Same for $y(t)$ using back-substitution.


